{-# OPTIONS --without-K --rewriting #-}

open import lib.Basics
open import lib.types.Sigma
open import lib.wild-cats.WildCats
open import Bicategory
open import AdjEq
open import Bicat-wild
open import Biadj
open import Pstransf-SIP
open import Univ-bc
open import Bicat-iso
open import Psftor-inverse
open import Psftor-laws
open import Biequiv
open import Badjbeqv-id

-- The notion of biadjoint biequivalence is fully coherent.

module Biadj-beqv where

open BicatStr {{...}}

open Pstrans
open BiequivStr-inst
open Biequiv-coh
open InvMod
open Equiv-wc

module _ {iâ‚ iâ‚‚ jâ‚ jâ‚‚} {C@(Câ‚€ , _) : Bicat jâ‚‚ iâ‚‚} {B@(Bâ‚€ , _) : Bicat jâ‚ iâ‚} where

  private
    instance
      Î¾C : BicatStr jâ‚‚ Câ‚€
      Î¾C = snd C
      Î¾B : BicatStr jâ‚ Bâ‚€
      Î¾B = snd B

  -- every biequivalence induces an equivalence of wild categories
  beqv-to-wniso : BiequivStr Î¾C Î¾B â†’ Equiv-wc (bc-to-wc B) (bc-to-wc C)
  ftorâ‚ (beqv-to-wniso be) = pf-to-wf (psftor-str (Î¨-L be))
  ftorâ‚‚ (beqv-to-wniso be) = pf-to-wf (psftor-str (Î¨-R be))
  fst (isoâ‚ (beqv-to-wniso be)) = ptr-to-ntr (Ï„â‚ be)
  snd (isoâ‚ (beqv-to-wniso be)) x = aeqv-to-weqv (lev-eqâ‚ be x)
  fst (isoâ‚‚ (beqv-to-wniso be)) = ptr-to-ntr (Ï„â‚‚ be)
  snd (isoâ‚‚ (beqv-to-wniso be)) x = aeqv-to-weqv (lev-eqâ‚‚ be x)

  open Psfunctor
  open PsftorStr
  open HAdjEquiv-wc

  baeqv-to-wniso : Î¾C biadj-bieqv Î¾B â†’ HAdjEquiv-wc (bc-to-wc B) (bc-to-wc C)
  ğ”¼ (baeqv-to-wniso (be , _)) = beqv-to-wniso be
  zig-zag (baeqv-to-wniso (be , ba)) x =
    ap (Î» m â†’ m â—» Î·â‚€ (Ï„â‚‚ be) (map-pf (Î¨-R be) x)) (Ï Î¾B (Fâ‚ (str-pf (Î¨-R be)) (Î·â‚€ (Ï„â‚ be) x)))  âˆ™
    Î·â‚€-âˆ¼ (Î¶Î¶ ba) x âˆ™
    ! (lamb Î¾B (idâ‚ Î¾B (map-pf (Î¨-R be) x)))

  -- Both pseudofunctors of a biadjoint biequivalence are fully faithful.

  baeqv-is-ff-R : ((be , _) : Î¾C biadj-bieqv Î¾B) â†’ (x y : Câ‚€) â†’ is-equiv (Fâ‚ (str-pf (Î¨-R be)) {x} {y})
  baeqv-is-ff-R bae _ _ = HAEquiv-wc-ff-R {C = bc-to-wc B} {D = bc-to-wc C} (baeqv-to-wniso bae)

  baeqv-is-ff-L : ((be , _) : Î¾C biadj-bieqv Î¾B) â†’ (x y : Bâ‚€) â†’ is-equiv (Fâ‚ (str-pf (Î¨-L be)) {x} {y})
  baeqv-is-ff-L bae _ _ = HAEquiv-wc-ff-L {C = bc-to-wc B} {D = bc-to-wc C} (baeqv-to-wniso bae)

  module _ {{uC : is-univ-bc-inst {{Î¾C}}}} {{uB : is-univ-bc-inst {{Î¾B}}}} where

    -- being a biadjoint biequivalence is a mere proposition
    abstract
      biadjequiv-is-prop : {R : Psfunctor {{Î¾C}} {{Î¾B}}} â†’ is-prop (is-biadj-bieqv R)
      biadjequiv-is-prop {R} = inhab-to-contr-is-prop Î» ((L , Î·) , (Îµ , _))
        â†’ Î£-level (psf-hi-rinv-contr {R = R} (L , (Îµ , Î·))) Î» Î·' â†’
          bae-rinv-cd-contr {R = R} {fst Î·'} (transport (Î» m â†’ psftor-str (m âˆ˜BC R) psf-â‰ƒ idpfBC)
            (psf-has-rinv-unique {R = R} (L , (Îµ , Î·)) {Râ‚ = L} {Râ‚‚ = fst Î·'} Î· (snd Î·')) Îµ) (snd Î·')

    is-biadj-bieqv-tot : Type (lmax (lmax (lmax iâ‚ iâ‚‚) jâ‚) jâ‚‚)
    is-biadj-bieqv-tot = Î£ (Psfunctor {{Î¾C}} {{Î¾B}}) is-biadj-bieqv

    bae-tot-â‰ƒ : Î¾C biadj-bieqv Î¾B â‰ƒ is-biadj-bieqv-tot
    bae-tot-â‰ƒ = equiv
      (Î» (bes , c) â†’ (Î¨-R bes) , (((Î¨-L bes) , (Î· bes)) , (Îµ bes , Î¶Î¶ c)))
      (Î» (ÏˆR , ((ÏˆL , eta) , (eps , zz))) â†’ (bequiv ÏˆL ÏˆR eps eta) , bieqvcoh zz)
      (Î» _ â†’ idp)
      Î» _ â†’ idp

module _ {i j} {Câ‚€ Bâ‚€ : Type i} {{Î¾C : BicatStr j Câ‚€}} {{Î¾B : BicatStr j Bâ‚€}}
  {{uC : is-univ-bc-inst {{Î¾C}}}} {{uB : is-univ-bc-inst {{Î¾B}}}} where

  private
  
    C : Bicat j i
    C = (Câ‚€ , Î¾C)

    B : Bicat j i
    B = (Bâ‚€ , Î¾B)

  bae-tot-iso : is-biadj-bieqv-tot â‰ƒ Î¾C iso-bc Î¾B
  bae-tot-iso = Î£-emap-r (Î» R â†’ props-BiImp-â‰ƒ {{biadjequiv-is-prop {R = R}}} {{iso-bc-is-prop {Ï† = R}}}
    (forw R) Î» iso â†’ backw (R , iso))
    where
    
      open Psfunctor
      forw : (R : Psfunctor {{Î¾C}} {{Î¾B}}) â†’ is-biadj-bieqv R â†’ is-iso-bc R
      fst (forw R ((L , ri) , li , _)) = is-eq (map-pf R) (map-pf L)
        (Î» b â†’ ! (ubc-ae-to-== ((Î·â‚€ (fst ri) b) , (snd ri b))))
        Î» c â†’ ubc-ae-to-== ((Î·â‚€ (fst li) c) , (snd li c))
      snd (forw R is-bae) = baeqv-is-ff-R (<â€“ bae-tot-â‰ƒ (R , is-bae))

      backw : {(_ , Î¾E) : Bicat j i} (iso : Î¾C iso-bc Î¾E) â†’
        {{_ : is-univ-bc-inst {{Î¾E}}}} â†’ is-biadj-bieqv {{Î¾B = Î¾E}} (fst iso)
      backw = bc-ind Î¾C (Î» E iso â†’ âˆ€ {{uE : is-univ-bc-inst {{snd E}}}} â†’
        is-biadj-bieqv {{Î¾B = snd E}} {{uC = uC}} {{uE}} (fst iso)) Î» {{uE}} â†’
          snd (â€“> (bae-tot-â‰ƒ {{uC = uC}} {{uC}}) biadj-bieuqiv-id)
          
  -- biadjoint equivalences are equivalent to isomorphisms, hence identities

  bae-iso-â‰ƒ : Î¾C biadj-bieqv Î¾B â‰ƒ Î¾C iso-bc Î¾B
  bae-iso-â‰ƒ = bae-tot-iso âˆ˜e bae-tot-â‰ƒ

  bae-==-â‰ƒ : (Î¾C biadj-bieqv Î¾B) â‰ƒ (C == B)
  bae-==-â‰ƒ = iso-bc-==-â‰ƒ âˆ˜e bae-tot-iso âˆ˜e bae-tot-â‰ƒ 

  -- Ïˆ-R induces an equality between bicategories
  baequiv-to-==-R : Î¾C biadj-bieqv Î¾B â†’ C == B
  baequiv-to-==-R bae = â€“> bae-==-â‰ƒ bae
